src/index.v
@@ -43,40 +43,54 @@ Definition projTI2 {C} {A : iType C} (P : forall i, A i -> Type) i
 
 Definition sigImply {C} {A : iType C} (P Q : forall i, A i -> Prop)
            (H : forall i x, P i x -> Q i x) i (x : sigI P i) : sigI Q i :=
-  match x with
-  | existI x p => existI x (H _ _ p)
-  end.
+  existI (projI1 x) (H _ _ (projI2 x)).
 
 Definition sigTImply {C} {A : iType C} (P Q : forall i, A i -> Type)
            (H : forall i x, P i x -> Q i x) i (x : sigTI P i) : sigTI Q i :=
-  match x with
-  | existTI x p => existTI x (H _ _ p)
-  end.
+  existTI (projTI1 x) (H _ _ (projTI2 x)).
 
 Definition sigImply_proj1 {C} {A : iType C} (P Q : forall i, A i -> Prop)
            (H : forall i x, P i x -> Q i x) i (x : sigI P i) :
   projI1 x = projI1 (sigImply _ H x).
 Proof.
-  destruct x. reflexivity.
+  reflexivity.
 Qed.
 
 Definition sigImply_proj2 {C} {A : iType C} (P Q : forall i, A i -> Prop)
            (H : forall i x, P i x -> Q i x) i (x : sigI P i) :
   projI2 (sigImply _ H x) = projI2 (sigImply _ H x).
 Proof.
-  destruct x. reflexivity.
+  reflexivity.
 Qed.
 
 Definition sigTImply_proj1 {C} {A : iType C} (P Q : forall i, A i -> Type)
            (H : forall i x, P i x -> Q i x) i (x : sigTI P i) :
   projTI1 x = projTI1 (sigTImply _ H x).
 Proof.
-  destruct x. reflexivity.
+  reflexivity.
 Qed.
 
 Definition sigTImply_proj2 {C} {A : iType C} (P Q : forall i, A i -> Type)
            (H : forall i x, P i x -> Q i x) i (x : sigTI P i) :
   projTI2 (sigTImply _ H x) = projTI2 (sigTImply _ H x).
 Proof.
-  destruct x. reflexivity.
+  reflexivity.
+Qed.
+
+Definition sigTimply A (P Q : A -> Type)
+           (H : forall a, P a -> Q a) (x : sigT P) : sigT Q :=
+  existT _ _ (H _ (projT2 x)).
+
+Definition sigTimply_proj1 A (P Q : A -> Type)
+           (H : forall a, P a -> Q a) (x : sigT P) :
+  projT1 x = projT1 (sigTimply _ H x).
+Proof.
+  reflexivity.
+Qed.
+
+Definition sigTimply_proj2 A (P Q : A -> Type)
+           (H : forall a, P a -> Q a) (x : sigT P) :
+  H _ (projT2 x) = projT2 (sigTimply _ H x).
+Proof.
+  reflexivity.
 Qed.
