src/hott.v
@@ -1,0 +1,37 @@
+Set Implicit Arguments.
+
+Record eqv (A B : Type) := Eqv {
+                               fn1 : A -> B;
+                               fn2 : B -> A;
+                               bij1 : forall a, fn2 (fn1 a) = a;
+                               bij2 : forall b, fn1 (fn2 b) = b;
+                             }.
+Notation "A ~ B" := (eqv A B) (at level 50).
+
+Goal True. constructor. Qed.
+
+Definition code_inl A B (a : A) (x : A + B) : Type :=
+  match x with
+  | inl a0 => (a = a0)
+  | inr b0 => False end.
+
+Lemma sum_eq_inl1 A B a x : (@eq (sum A B) (inl a) x) -> code_inl a x.
+Proof.
+  intro.
+  apply (eq_rect (inl a) (code_inl a) eq_refl x H).
+Defined.
+
+Lemma sum_eq_inl2 A B a x : code_inl a x -> (@eq (sum A B) (inl a) x).
+Proof.
+  intro.
+  destruct x.
+  - apply (f_equal inl X).
+  - destruct X.
+Defined.
+
+Lemma sum_eq A B a x : (@eq (sum A B) (inl a) x) ~ (code_inl a x).
+Proof.
+  apply (Eqv (@sum_eq_inl1 _ _ _ _) (@sum_eq_inl2 _ _ _ _));
+    unfold sum_eq_inl1, sum_eq_inl2, f_equal.
+  - intro. destruct x. simpl. admit.
+Admitted.
