src/iinductive2.v
@@ -1,0 +1,298 @@
+Require Import FunctionalExtensionality.
+Require Import Program.
+
+Set Implicit Arguments.
+
+Require Import index wf IFunctor ISPFunctor.
+
+Section INDUCTIVE.
+
+  Variable O : Type.
+  Variable F : O -> (O -> Type) -> Type.
+
+  Context `{H : forall c, SPFunctor (F c)}.
+  Variable X : (iType O).
+
+  Inductive Mu : O -> Type :=
+  | Con' o : Container (@P _ _ (H o)) Mu -> Mu o.
+
+  Definition Con o (fx : F o Mu) : Mu o := Con' o (NT _ fx).
+
+  Definition Des' o (m : Mu o) : Container (@P _ _ (H o)) Mu :=
+    match m with
+    | Con' o s => s end.
+
+  Definition Des o (m : Mu o) : F o Mu := NTinv _ (Des' m).
+
+  Lemma eta_expand2 : forall o (x : Mu o), Con (Des x) = x.
+  Proof.
+    intros. unfold Des, Con. rewrite BIJECTION2.
+    destruct x. reflexivity.
+  Qed.
+
+  Lemma eta_expand1 : forall o (x : F o Mu), Des (Con x) = x.
+  Proof.
+    intros. unfold Des, Con.
+    rewrite <- BIJECTION1.
+    destruct (NT Mu x). reflexivity.
+  Qed.
+
+  Definition ord : forall o1, Mu o1 -> forall o2, Mu o2 -> Prop :=
+   fun o1 m1 o2 m2 => mem (Des' m2) m1.
+
+  Lemma ord_wf : iwell_founded ord.
+  Proof.
+    unfold iwell_founded. fix 2.
+    intros o2 m2. constructor.
+    intros o1 m1 ORD. destruct ORD.
+    rewrite <- H0. apply ord_wf.
+  Qed.
+
+  Definition ord_c := iclos_transn1 ord.
+
+  Lemma ord_correct : forall o1 (m : Mu o1) o2 (fx : F o2 Mu),
+      @mem O (F o2) _ Mu fx o1 m <-> ord m (Con fx).
+  Proof.
+    intros. rewrite MEM_COMMUTE. reflexivity.
+  Qed.
+
+  Lemma ord_c_wf : iwell_founded ord_c.
+  Proof.
+    apply wf_iclos_trans. apply ord_wf.
+  Qed.
+
+  Lemma ord_transitive o1 o2 o3 (x : Mu o1) (y : Mu o2) (z : Mu o3) :
+    ord_c x y -> ord_c y z -> ord_c x z.
+  Proof.
+    apply iclos_transn1_transitive.
+  Qed.
+
+  Definition rec (P : forall o, Mu o -> Type)
+             (FIX : forall o1 (m1 : Mu o1), 
+                 (forall o2 (m2 : Mu o2), ord_c m2 m1 -> P o2 m2) -> P o1 m1) :
+    forall o (m : Mu o), P o m :=
+    iFix ord_c_wf P FIX.
+
+  Definition rec_simpl1 (P : forall o, Type)
+             (FIX : forall o1 (m1 : Mu o1), 
+                 (forall o2 (m2 : Mu o2), ord_c m2 m1 -> P o2) -> P o1) :
+    forall o, Mu o -> P o :=
+    rec _ FIX.
+
+  Definition rec_simpl2 T
+             (FIX : forall o1 (m1 : Mu o1), 
+                 (forall o2 (m2 : Mu o2), ord_c m2 m1 -> T) -> T) :
+    forall o, Mu o -> T :=
+    rec_simpl1 _ FIX.
+
+  Lemma rec_red (P : forall o, Mu o -> Type)
+        (FIX : forall o1 (m1 : Mu o1), 
+            (forall o2 (m2 : Mu o2), ord_c m2 m1 -> P o2 m2) -> P o1 m1)
+        o (fx : F o  Mu) :
+    rec _ FIX (Con fx) = FIX _ (Con fx) (fun _ fy _ => rec _ FIX fy).
+  Proof.
+    apply iFix_eq.
+  Qed.
+
+  Lemma rec_simpl1_red (P : forall o, Type)
+        (FIX : forall o1 (m1 : Mu o1), 
+            (forall o2 (m2 : Mu o2), ord_c m2 m1 -> P o2) -> P o1) 
+        o (fx : F o Mu) :
+    rec_simpl1 _ FIX (Con fx) = FIX _ (Con fx) (fun _ fy _ => rec_simpl1 _ FIX fy).
+  Proof.
+    apply (rec_red _ FIX fx).
+  Qed.
+
+  Lemma rec_simpl2_red T
+        (FIX : forall o1 (m1 : Mu o1), 
+            (forall o2 (m2 : Mu o2), ord_c m2 m1 -> T) -> T)
+        o (fx : F o Mu) :
+    rec_simpl2 FIX (Con fx) = FIX _ (Con fx) (fun _ fy _ => rec_simpl2 FIX fy).
+  Proof.
+    apply (rec_simpl1_red _ FIX fx).
+  Qed.
+
+  Definition induction_principle (P : forall o, Mu o -> Prop)
+             (FIX : forall o1 (m1 : Mu o1), 
+                 (forall o2 (m2 : Mu o2), ord m2 m1 -> P o2 m2) -> P o1 m1) :
+    forall o (m : Mu o), P o m.
+  Proof.
+    apply (iFix ord_wf P FIX).
+  Qed.
+
+  Definition str_induction_principle (P : forall o, Mu o -> Prop)
+             (FIX : forall o1 (m1 : Mu o1), 
+                 (forall o2 (m2 : Mu o2), ord_c m2 m1 -> P o2 m2) -> P o1 m1) :
+    forall o (m : Mu o), P o m.
+  Proof.
+    apply (iFix ord_c_wf P FIX).
+  Qed.
+
+  Definition mem_induction_principle (P : forall o, Mu o -> Prop)
+             (FIX : forall o1 (fx : F o1 Mu), 
+                 (forall o2 (m : Mu o2), mem fx m -> P _ m) -> P _ (Con fx)) :
+    forall o (m : Mu o), P o m.
+  Proof.
+    apply induction_principle.
+    intros o1 m1. destruct (eta_expand2 m1).
+    intros. apply FIX.
+    intros. apply H0, ord_correct, H1.
+  Qed.
+
+  Lemma ord_lemma o (m : Mu o)
+    : forall (i : O) (x : Mu i), mem (Des m) x -> ord_c x m.
+  Proof.
+    intros i x MEM.
+    rewrite <- eta_expand2. apply itn1_step, ord_correct, MEM.
+  Qed.
+
+  Definition Des_ord o (m : Mu o) : F o (sigI (fun i x => @ord_c i x _ m)) :=
+    @map _ (F o) _ _ _ (sigImply _ (ord_lemma m)) (tag _ (Des m)).
+
+  Lemma Des_ord_correct o (fx : F o Mu)
+    : map (@projI1 _ _ _) (Des_ord (Con fx)) = fx.
+  Proof.
+    unfold Des_ord. rewrite MAP_COMPOSE.
+    simpl. rewrite TAG. apply eta_expand1.
+  Qed.
+
+  Definition prim_rec1 (P : forall (o : O), Type)
+             (FIX : forall o, F o P -> P o) :=
+    rec_simpl1 P (fun o1 m1 f => FIX _ (map (fun o fx => f _ (projI1 fx) (projI2 fx))
+                                            (Des_ord m1))).
+
+  Lemma prim_rec1_red (P : forall (o : O), Type)
+        (FIX : forall o, F o P -> P o) o (fx : F o Mu) :
+    prim_rec1 FIX (Con fx) = FIX o (map (prim_rec1 FIX) fx).
+  Proof.
+    unfold prim_rec1.
+    rewrite rec_simpl1_red.
+    pattern fx at 5.
+    rewrite <- (Des_ord_correct fx).
+    rewrite MAP_COMPOSE. reflexivity.
+  Qed.    
+
+  Definition prim_rec2 T
+             (FIX : forall o, F o (fun _ => T) -> T) :
+    forall o, Mu o -> T :=
+    prim_rec1 FIX.
+  
+  Lemma prim_rec2_red T (FIX : forall o, F o (fun _ => T) -> T)
+        o (fx : F o Mu) :
+    prim_rec2 FIX (Con fx) = FIX _ (map (prim_rec2 FIX) fx).
+  Proof.
+    apply (prim_rec1_red FIX).
+  Qed.
+
+
+
+(*
+
+  Definition rec_mem' (T : forall o, Mu o -> Type)
+             (FIX : forall o1 m1, 
+                 (forall o2 m2, mem m1 m2 -> T o2 m2) -> T o1 (Con' o1 m1)) :
+    forall o (m : Mu o), T o m.
+    apply rec. intros o1 m1 f.
+    destruct m1. apply FIX.
+    intros o2 m2 MEM. apply f, itn1_step, MEM.
+  Defined.
+
+  Lemma rec_mem'_red (T : forall o, Mu o -> Type)
+             (FIX : forall o1 m1, 
+                 (forall o2 m2, mem m1 m2 -> T o2 m2) -> T o1 (Con' o1 m1)) :
+    forall o m,
+      rec_mem' T FIX (Con' o m) = FIX _ m (fun o2 m2 _ => rec_mem' T FIX m2).
+  Proof.  
+    intros. apply iFix_eq.
+  Qed.
+
+  (* this is the most general one!! however i'm not sure it can be proven without K *)
+  Definition rec_mem2 (T : forall o, Mu o -> Type)
+             (FIX : forall o1 (m1 : F o1 Mu), 
+                 (forall o2 m2, mem m1 m2 -> T o2 m2) -> T o1 (Con m1)) :
+    forall o (m : Mu o), T o m.
+    apply rec_mem'.
+    intros. specialize (FIX _ (NTinv _ m1)).
+
+    unfold Con in FIX. rewrite BIJECTION2 in FIX. apply FIX.
+    intros. apply X0. apply MEM_COMMUTE in H0. rewrite BIJECTION2 in H0. apply H0.
+  Defined.
+
+  Lemma rec_mem_red2 (T : forall o, Mu o -> Type)
+        (FIX : forall o1 (m1 : F o1 Mu), 
+            (forall o2 (m2 : Mu o2), mem m1 m2 -> T o2 m2) -> T o1 (Con m1)) :
+    forall o (m : F o Mu),
+      rec_mem2 T FIX (Con m) = FIX _ m (fun o2 m2 _ => rec_mem2 T FIX m2).
+    intros. unfold Con. unfold rec_mem2 at 1. simpl.
+    rewrite rec_mem'_red. simpl.
+    
+    set (f := fun m' : F o Mu => (fun (o2 : O) (m2 : Mu o2) (_ : mem m' m2) => rec_mem2 T FIX m2)).
+
+    assert (eq_rect (NT Mu (NTinv Mu (NT Mu m)))
+    (fun c : Container P Mu =>
+     (forall (o2 : O) (m2 : Mu o2), mem (NTinv Mu (NT Mu m)) m2 -> T o2 m2) ->
+     T o (Con' o c)) (FIX o (NTinv Mu (NT Mu m))) (NT Mu m) 
+    (BIJECTION2 Mu (NT Mu m)) (f (NTinv Mu (NT Mu m))) =
+  FIX o m (f m)); [| apply H0].
+
+    simpl. remember (BIJECTION2 Mu (NT Mu m)). 
+  Admitted.
+
+  Lemma rec_mem_lemma o1 (m1 : Mu o1) o2 (m2 : Mu o2) :
+    mem (Des m1) m2 -> ord_c m2 m1.
+  Proof.
+    intro MEM. rewrite <- eta_expand2.
+    apply itn1_step, ord_correct, MEM.
+  Qed.
+
+  Definition rec_mem (T : forall o, Mu o -> Type)
+             (FIX : forall o1 (m1 : F o1 Mu), 
+                 (forall o2 (m2 : Mu o2), mem m1 m2 -> T o2 m2) -> T o1 (Con m1)) :
+    forall o (m : Mu o), T o m.
+    apply rec. intros o1 m1 f.
+
+    
+    rewrite <- eta_expand2. apply FIX. 
+
+    intros o2 m2 MEM. apply f. apply (rec_mem_lemma _ _ MEM).
+  Defined.
+
+  Lemma rec_mem_red (T : forall o, Mu o -> Type)
+        (FIX : forall o1 (m1 : F o1 Mu), 
+            (forall o2 (m2 : Mu o2), mem m1 m2 -> T o2 m2) -> T o1 (Con m1)) :
+    forall o (m : F o Mu),
+      rec_mem T FIX (Con m) = FIX _ m (fun o2 m2 _ => rec_mem T FIX m2).
+
+
+    intros. unfold rec_mem at 1. rewrite rec_red. simpl.
+    set (f := fun (m' : F o Mu) => fun (o2 : O) (m2 : Mu o2) (_ : mem m' m2) => rec_mem T FIX m2).
+    assert (eq_rect (Con (Des (Con m))) (T o)
+                    (FIX o (Des (Con m)) (f (Des (Con m)))) (Con m) (eta_expand2 (Con m)) =
+            FIX o m (f m)).
+    - remember (eta_expand2 (Con m)).
+
+      
+      assert (m' : Mu o). admit.
+      assert (Des m' = m). admit.
+      destruct H0. simpl. 
+
+      admit.
+
+  Definition Des2 : forall o, Mu o -> F o Mu :=
+    rec_mem (fun o _ => F o Mu) (fun _ m _ => m). 
+
+  Goal True. apply I. Qed.
+
+  Lemma Des2_eta1 : forall o (x : Mu o), Con (Des2 x) = x.
+  Proof.
+    apply rec_mem. intros o1 m1 FIX.
+    unfold Des2. rewrite rec_mem_red. reflexivity.
+  Qed.
+
+  Lemma Des2_eta2 : forall o (fx : F o Mu), Des2 (Con fx) = fx.
+  Proof.
+    intros. unfold Des2. rewrite rec_mem_red. reflexivity. 
+  Qed.
+*)
+
+End INDUCTIVE.
